Refactor the refinement predicate (#120)

correctness/RegexCorrectness/Backtracker/Refinement.lean
@@ -5,132 +5,100 @@ set_option autoImplicit false
 
 open Regex (NFA)
 open Regex.Data (BitMatrix BoundedIterator)
-open Regex.Strategy (refineUpdate refineUpdateOpt refineUpdates materializeUpdates)
+open Regex.Strategy (materializeUpdates)
 open String (Pos)
 namespace Regex.Backtracker
 
 variable {nfa : NFA} {wf : nfa.WellFormed} {startIdx maxIdx bufferSize : Nat}
 
-def StackEntry.Refines (entryH : StackEntry HistoryStrategy nfa startIdx maxIdx) (entryB : StackEntry (BufferStrategy bufferSize) nfa startIdx maxIdx) : Prop :=
-  refineUpdate entryH.update entryB.update ∧ entryH.state = entryB.state ∧ entryH.it = entryB.it
+def StackEntry.materialize (entryH : StackEntry HistoryStrategy nfa startIdx maxIdx) : StackEntry (BufferStrategy bufferSize) nfa startIdx maxIdx :=
+  ⟨materializeUpdates bufferSize entryH.update, entryH.state, entryH.it⟩
 
-theorem StackEntry.Refines.simpL {update state it} {entryB : StackEntry (BufferStrategy bufferSize) nfa startIdx maxIdx} (ref : StackEntry.Refines ⟨update, state, it⟩ entryB) :
-  entryB = ⟨entryB.update, state, it⟩ := by
-  unfold StackEntry.Refines at ref
-  simp_all
+def materializeStack (stackH : List (StackEntry HistoryStrategy nfa startIdx maxIdx)) : List (StackEntry (BufferStrategy bufferSize) nfa startIdx maxIdx) :=
+  stackH.map StackEntry.materialize
 
-theorem StackEntry.Refines.mk {update} {state state' : Fin nfa.nodes.size} {it it' : BoundedIterator startIdx maxIdx} {entryB : StackEntry (BufferStrategy bufferSize) nfa startIdx maxIdx}
-  (ref : StackEntry.Refines ⟨update, state, it⟩ entryB) :
-  StackEntry.Refines ⟨update, state', it'⟩ ⟨entryB.update, state', it'⟩ := by
-  simp [Refines] at ref
-  simp [Refines, ref]
+@[simp]
+theorem materializeStack.nil : materializeStack [] = ([] : List (StackEntry (BufferStrategy bufferSize) nfa startIdx maxIdx)) := rfl
 
-theorem StackEntry.Refines.empty {state : Fin nfa.nodes.size} {it : BoundedIterator startIdx maxIdx} : StackEntry.Refines ⟨HistoryStrategy.empty, state, it⟩ ⟨(BufferStrategy bufferSize).empty, state, it⟩ := by
-  simp [Refines]
+@[simp]
+theorem materializeStack.cons {entryH stackH} :
+  materializeStack (entryH :: stackH) = (StackEntry.materialize entryH :: materializeStack stackH : List (StackEntry (BufferStrategy bufferSize) nfa startIdx maxIdx)) := rfl
 
-inductive RefineStack : List (StackEntry HistoryStrategy nfa startIdx maxIdx) → List (StackEntry (BufferStrategy bufferSize) nfa startIdx maxIdx) → Prop where
-  | nil : RefineStack [] []
-  | cons (entryH entryB stackH stackB) : entryH.Refines entryB → RefineStack stackH stackB → RefineStack (entryH :: stackH) (entryB :: stackB)
+def materializeResultAux (resultH : Option (List (Nat × Pos)) × BitMatrix nfa.nodes.size (maxIdx + 1 - startIdx)) : Option (Buffer bufferSize) × BitMatrix nfa.nodes.size (maxIdx + 1 - startIdx) :=
+  ⟨resultH.1.map (materializeUpdates bufferSize), resultH.2⟩
 
-def Refines (resultH : Option (List (Nat × Pos)) × BitMatrix nfa.nodes.size (maxIdx + 1 - startIdx)) (resultB : Option (Buffer bufferSize) × BitMatrix nfa.nodes.size (maxIdx + 1 - startIdx)) : Prop :=
-  refineUpdateOpt resultH.1 resultB.1 ∧ resultH.2 = resultB.2
+def materializeResult (resultH : Option (List (Nat × Pos))) : Option (Buffer bufferSize) :=
+  resultH.map (materializeUpdates bufferSize)
 
 theorem captureNextAux.pushNext.refines {nfa wf startIdx maxIdx bufferSize stackH stackB updateH updateB state it}
-  (refEntry : StackEntry.Refines ⟨updateH, state, it⟩ ⟨updateB, state, it⟩) (refStack : RefineStack stackH stackB) :
-  RefineStack (captureNextAux.pushNext HistoryStrategy nfa wf startIdx maxIdx stackH updateH state it) (captureNextAux.pushNext (BufferStrategy bufferSize) nfa wf startIdx maxIdx stackB updateB state it) := by
+  (refEntry : StackEntry.materialize ⟨updateH, state, it⟩ = ⟨updateB, state, it⟩) (refStack : materializeStack stackH = stackB) :
+  materializeStack (captureNextAux.pushNext HistoryStrategy nfa wf startIdx maxIdx stackH updateH state it) = captureNextAux.pushNext (BufferStrategy bufferSize) nfa wf startIdx maxIdx stackB updateB state it := by
   cases stackH, updateH, state, it using captureNextAux.pushNext.fun_cases' HistoryStrategy nfa wf startIdx maxIdx with
   | done stackH updateH state it hn => simp [pushNext.done hn, refStack]
   | fail stackH updateH state it hn => simp [pushNext.fail hn, refStack]
   | epsilon stackH updateH state it state' hn =>
-    simp [pushNext.epsilon hn]
-    exact .cons _ _ _ _ refEntry.mk refStack
+    simp [StackEntry.materialize] at refEntry
+    simp [pushNext.epsilon hn, StackEntry.materialize, refStack, refEntry]
   | split stackH updateH state it state₁ state₂ hn =>
-    simp [pushNext.split hn]
-    exact .cons _ _ _ _ refEntry.mk (.cons _ _ _ _ refEntry.mk refStack)
+    simp [StackEntry.materialize] at refEntry
+    simp [pushNext.split hn, StackEntry.materialize, refStack, refEntry]
   | save stackH updateH state it offset state' hn =>
-    -- This is the only interesting case, where we update the history/buffer
-    simp [pushNext.save hn]
-    refine .cons _ _ _ _ ?_ refStack
-    simp [StackEntry.Refines, refineUpdate] at refEntry
-    simp [StackEntry.Refines, refineUpdate, HistoryStrategy, BufferStrategy, refEntry]
+    simp [StackEntry.materialize] at refEntry
+    simp [pushNext.save hn, StackEntry.materialize, refStack, refEntry]
   | anchor_pos stackH updateH state it a state' hn ht =>
-    simp [pushNext.anchor_pos hn ht]
-    exact .cons _ _ _ _ refEntry.mk refStack
-  | anchor_neg stackH updateH state it a state' hn ht => simp [pushNext.anchor_neg hn ht, refStack]
+    simp [StackEntry.materialize] at refEntry
+    simp [pushNext.anchor_pos hn ht, StackEntry.materialize, refStack, refEntry]
+  | anchor_neg stackH updateH state it a state' hn ht =>
+    simp [pushNext.anchor_neg hn ht, refStack]
   | char_pos stackH updateH state it c state' hn hnext hc =>
-    simp [pushNext.char_pos hn hnext hc]
-    exact .cons _ _ _ _ refEntry.mk refStack
-  | char_neg stackH updateH state it c state' hn h => simp [pushNext.char_neg hn h, refStack]
+    simp [StackEntry.materialize] at refEntry
+    simp [pushNext.char_pos hn hnext hc, StackEntry.materialize, refStack, refEntry]
+  | char_neg stackH updateH state it c state' hn h =>
+    simp [pushNext.char_neg hn h, refStack]
   | sparse_pos stackH updateH state it cs state' hn hnext hc =>
-    simp [pushNext.sparse_pos hn hnext hc]
-    exact .cons _ _ _ _ refEntry.mk refStack
-  | sparse_neg stackH updateH state it cs state' hn h => simp [pushNext.sparse_neg hn h, refStack]
+    simp [StackEntry.materialize] at refEntry
+    simp [pushNext.sparse_pos hn hnext hc, StackEntry.materialize, refStack, refEntry]
+  | sparse_neg stackH updateH state it cs state' hn h =>
+    simp [pushNext.sparse_neg hn h, refStack]
 
-theorem captureNextAux.refines (nfa wf startIdx maxIdx bufferSize visited) {stackH stackB} (refStack : RefineStack stackH stackB) :
-  Refines (captureNextAux HistoryStrategy nfa wf startIdx maxIdx visited stackH) (captureNextAux (BufferStrategy bufferSize) nfa wf startIdx maxIdx visited stackB) := by
+theorem captureNextAux.refines (nfa wf startIdx maxIdx bufferSize visited) {stackH stackB} (refStack : materializeStack stackH = stackB) :
+  materializeResultAux (captureNextAux HistoryStrategy nfa wf startIdx maxIdx visited stackH) = captureNextAux (BufferStrategy bufferSize) nfa wf startIdx maxIdx visited stackB := by
   induction visited, stackH using captureNextAux.induct' HistoryStrategy nfa wf startIdx maxIdx generalizing stackB with
   | base visited =>
-    cases refStack with
-    | nil => simp [captureNextAux_base, Refines, refineUpdateOpt]
+    simp at refStack
+    simp [refStack, captureNextAux_base, materializeResultAux]
   | visited visited update state' it stackH mem ih =>
-    cases refStack with
-    | cons entryH entryB stackH stackB refEntry refStack =>
-      rw [refEntry.simpL]
-      simp [captureNextAux_visited mem]
-      exact ih refStack
+    simp at refStack
+    simpa [←refStack, StackEntry.materialize, captureNextAux_visited mem] using ih rfl
   | done visited update state' it stackH mem hn =>
-    cases refStack with
-    | cons entryH entryB stackH stackB refEntry refStack =>
-      rw [refEntry.simpL]
-      simp [captureNextAux_done mem hn, Refines, refineUpdateOpt, refEntry.1]
+    simp at refStack
+    simp [←refStack, StackEntry.materialize, captureNextAux_done mem hn, materializeResultAux]
   | next visited update state' it stackH mem hn ih =>
-    cases refStack with
-    | cons entryH entryB stackH stackB refEntry refStack =>
-      rw [refEntry.simpL]
-      simp [captureNextAux_next mem hn]
-      exact ih (pushNext.refines (refEntry.simpL ▸ refEntry) refStack)
+    simp at refStack
+    simp [←refStack, StackEntry.materialize, captureNextAux_next mem hn]
+    exact ih (pushNext.refines rfl rfl)
 
 theorem captureNext.go.refines (nfa wf startIdx bufferSize bit visited) :
-  refineUpdateOpt (captureNext.go HistoryStrategy nfa wf startIdx maxIdx bit visited) (captureNext.go (BufferStrategy bufferSize) nfa wf startIdx maxIdx bit visited) := by
+  materializeResult (captureNext.go HistoryStrategy nfa wf startIdx maxIdx bit visited) = captureNext.go (BufferStrategy bufferSize) nfa wf startIdx maxIdx bit visited := by
   induction bit, visited using captureNext.go.induct' HistoryStrategy nfa wf startIdx maxIdx with
   | found bit visited updateH visitedH hauxH =>
-    let entryH : StackEntry HistoryStrategy nfa startIdx maxIdx := ⟨HistoryStrategy.empty, ⟨nfa.start, wf.start_lt⟩, bit⟩
-    let entryB : StackEntry (BufferStrategy bufferSize) nfa startIdx maxIdx := ⟨(BufferStrategy bufferSize).empty, ⟨nfa.start, wf.start_lt⟩, bit⟩
-    have refStack : RefineStack [entryH] [entryB] := .cons entryH entryB [] [] .empty .nil
-    have refResult := captureNextAux.refines nfa wf startIdx maxIdx bufferSize visited refStack
-    match hauxB : captureNextAux (BufferStrategy bufferSize) nfa wf startIdx maxIdx visited [entryB] with
-    | (.some updateB, visitedB) =>
-      simp [Refines, entryH, hauxH, hauxB, refineUpdateOpt] at refResult
-      simp [captureNext.go_found hauxH, captureNext.go_found hauxB, refineUpdateOpt, refResult]
-    | (.none, _) => simp [Refines, entryH, hauxH, hauxB, refineUpdateOpt] at refResult
+    have hauxB := captureNextAux.refines nfa wf startIdx maxIdx bufferSize visited rfl (stackB := materializeStack [⟨HistoryStrategy.empty, ⟨nfa.start, wf.start_lt⟩, bit⟩])
+    simp [↓hauxH, materializeResultAux] at hauxB
+    simp [captureNext.go_found hauxH, captureNext.go_found hauxB.symm, materializeResult]
   | not_found_next bit visited visitedH hauxH hnext ih =>
-    let entryH : StackEntry HistoryStrategy nfa startIdx maxIdx := ⟨HistoryStrategy.empty, ⟨nfa.start, wf.start_lt⟩, bit⟩
-    let entryB : StackEntry (BufferStrategy bufferSize) nfa startIdx maxIdx := ⟨(BufferStrategy bufferSize).empty, ⟨nfa.start, wf.start_lt⟩, bit⟩
-    have refStack : RefineStack [entryH] [entryB] := .cons entryH entryB [] [] .empty .nil
-    have refResult := captureNextAux.refines nfa wf startIdx maxIdx bufferSize visited refStack
-    match hauxB : captureNextAux (BufferStrategy bufferSize) nfa wf startIdx maxIdx visited [entryB] with
-    | (.some _, _) => simp [Refines, entryH, hauxH, hauxB, refineUpdateOpt] at refResult
-    | (.none, visitedB) =>
-      simp [Refines, entryH, hauxH, hauxB, refineUpdateOpt] at refResult
-      simp [captureNext.go_not_found_next hauxH hnext, captureNext.go_not_found_next hauxB hnext]
-      exact refResult ▸ ih
+    have hauxB := captureNextAux.refines nfa wf startIdx maxIdx bufferSize visited rfl (stackB := materializeStack [⟨HistoryStrategy.empty, ⟨nfa.start, wf.start_lt⟩, bit⟩])
+    simp [↓hauxH, materializeResultAux] at hauxB
+    simpa [captureNext.go_not_found_next hauxH hnext, captureNext.go_not_found_next hauxB.symm hnext] using ih
   | not_found_end bit visited visitedH hauxH hnext =>
-    let entryH : StackEntry HistoryStrategy nfa startIdx maxIdx := ⟨HistoryStrategy.empty, ⟨nfa.start, wf.start_lt⟩, bit⟩
-    let entryB : StackEntry (BufferStrategy bufferSize) nfa startIdx maxIdx := ⟨(BufferStrategy bufferSize).empty, ⟨nfa.start, wf.start_lt⟩, bit⟩
-    have refStack : RefineStack [entryH] [entryB] := .cons entryH entryB [] [] .empty .nil
-    have refResult := captureNextAux.refines nfa wf startIdx maxIdx bufferSize visited refStack
-    match hauxB : captureNextAux (BufferStrategy bufferSize) nfa wf startIdx maxIdx visited [entryB] with
-    | (.some _, _) => simp [Refines, entryH, hauxH, hauxB, refineUpdateOpt] at refResult
-    | (.none, visitedB) =>
-      simp [Refines, entryH, hauxH, hauxB, refineUpdateOpt] at refResult
-      simp [captureNext.go_not_found_end hauxH hnext, captureNext.go_not_found_end hauxB hnext, refineUpdateOpt]
+    have hauxB := captureNextAux.refines nfa wf startIdx maxIdx bufferSize visited rfl (stackB := materializeStack [⟨HistoryStrategy.empty, ⟨nfa.start, wf.start_lt⟩, bit⟩])
+    simp [↓hauxH, materializeResultAux] at hauxB
+    simp [captureNext.go_not_found_end hauxH hnext, captureNext.go_not_found_end hauxB.symm hnext, materializeResult]
 
 theorem captureNext.refines (nfa wf bufferSize it) :
-  refineUpdateOpt (captureNext HistoryStrategy nfa wf it) (captureNext (BufferStrategy bufferSize) nfa wf it) := by
+  materializeResult (captureNext HistoryStrategy nfa wf it) = captureNext (BufferStrategy bufferSize) nfa wf it := by
   if le : it.pos ≤ it.toString.endPos then
-    simp [captureNext_le le]
-    exact (captureNext.go.refines nfa wf it.pos.byteIdx bufferSize ⟨it, Nat.le_refl _, le, rfl⟩ (BitMatrix.zero _ _))
+    simpa [captureNext_le le] using captureNext.go.refines nfa wf it.pos.byteIdx bufferSize ⟨it, Nat.le_refl _, le, rfl⟩ (BitMatrix.zero _ _)
   else
-    simp [captureNext_not_le le, refineUpdateOpt]
+    simp [captureNext_not_le le, materializeResult]
 
 end Regex.Backtracker
